MutableOrderedMap WIP

lib/MutableOrderedMap.dfy
@@ -1,10 +1,13 @@
 include "NativeTypes.dfy"
 include "Option.dfy"
-// include "sequences.dfy"
+include "sequences.dfy"
 // include "Sets.dfy"
 // include "SetBijectivity.dfy"
 
 abstract module MutableOrderedMap {
+  import opened Options
+  import opened Sequences
+
   type K(==)
   type V(==)
   function method LessEquals(a: K, b: K): bool
@@ -12,8 +15,6 @@ abstract module MutableOrderedMap {
   function method LessThan(a: K, b: K): bool {
     LessEquals(a, b) && !Equals(a, b)
   }
-
-  import opened Options
 
   datatype TwoThreeNodeRef = Internal(internal: InternalTwoThreeNode) | Leaf(leaf: LeafTwoThreeNode)
 
@@ -43,6 +44,45 @@ abstract module MutableOrderedMap {
     }
   }
 
+  predicate LeftSmallerThanRight(left: map<K, V>, right: map<K, V>)
+  {
+    && (forall l, r :: l in left && r in right ==> LessThan(l, r))
+  }
+
+  // lemma LeftSmallerThanRightTransitive(mapA: map<K, V>, mapB: map<K, V>, mapC: map<K, V>)
+  //   requires LeftSmallerThanRight(mapA, mapB)
+  //   requires LeftSmallerThanRight(mapB, mapC)
+  //   ensures LeftSmallerThanRight(mapA, mapC)
+  // {
+  //   forall a, c | a in mapA && c in mapC
+  //   ensures LessThan(a, c)
+  //   {
+  //   }
+  // }
+
+  lemma LeftSmallerThanRightImpliesDisjunctKeySets(left: map<K, V>, right: map<K, V>)
+    requires LeftSmallerThanRight(left, right)
+    ensures left.Keys !! right.Keys
+  {
+    if exists k :: k in left.Keys && k in right.Keys {
+      var k :| k in left.Keys && k in right.Keys;
+      assert exists k :: k in left.Keys && k in right.Keys && !LessThan(k, k);
+      assert false;
+    }
+    assert left.Keys !! right.Keys;
+  }
+
+  function InterpretData(data: seq<(K, V)>): (result: map<K, V>)
+    requires forall i, j :: 0 <= i < |data| && 0 <= j < |data| && data[i].0 == data[j].0 ==> i == j
+    ensures forall i :: 0 <= i < |data| ==> data[i].0 in result && result[data[i].0] == data[i].1
+  {
+    if |data| == 0 then
+      map[]
+    else
+      var (k, v) := Last(data);
+      InterpretData(DropLast(data))[k := v]
+  }
+
   class InternalTwoThreeNode {
     var Data: array<(K, V)>;
     var Children: array<TwoThreeNodeRef>;
@@ -60,7 +100,7 @@ abstract module MutableOrderedMap {
       && Repr == (ReprOf(Children[0]) + ReprOf(Children[1]) +
           if Children.Length == 3 then ReprOf(Children[2]) else {})
       && (forall c1, c2 :: 0 <= c1 < c2 < Children.Length
-          ==> (forall l, r :: l in ContentsOf(Children[c1]) && r in ContentsOf(Children[c2]) ==> LessThan(l, r)))
+          ==> LeftSmallerThanRight(ContentsOf(Children[c1]), ContentsOf(Children[c2])))
       && (forall d, c :: 0 <= d < Data.Length && 0 <= c < Children.Length
           ==> Data[d].0 !in ContentsOf(Children[c]).Keys)
       && (forall k :: k in Contents ==> (
@@ -72,6 +112,9 @@ abstract module MutableOrderedMap {
     }
 
     constructor (left: TwoThreeNodeRef, datum: (K, V), right: TwoThreeNodeRef)
+      requires LeftSmallerThanRight(ContentsOf(left), InterpretData([datum]))
+      requires LeftSmallerThanRight(InterpretData([datum]), ContentsOf(right))
+      requires LeftSmallerThanRight(ContentsOf(left), ContentsOf(right))
       ensures Inv()
     {
       var newData := [datum];
@@ -80,6 +123,21 @@ abstract module MutableOrderedMap {
       Children := new [2] (i requires 0 <= i < 2 => newChildren[i]);
 
       Repr := ReprOf(left) + ReprOf(right);
+
+      new;
+
+      assert forall c1, c2 :: 0 <= c1 < c2 < Children.Length
+          ==> LeftSmallerThanRight(ContentsOf(Children[c1]), ContentsOf(Children[c2]));
+      LeftSmallerThanRightImpliesDisjunctKeySets(ContentsOf(left), InterpretData([datum]));
+      LeftSmallerThanRightImpliesDisjunctKeySets(InterpretData([datum]), ContentsOf(right));
+      assert forall d, c :: 0 <= d < Data.Length && 0 <= c < Children.Length
+          ==> Data[d].0 !in ContentsOf(Children[c]).Keys;
+      assert forall k :: k in Contents ==> (
+          || (exists c ::
+              && 0 <= c < Children.Length
+              && var cnt := ContentsOf(Children[c]);
+              && k in cnt && cnt[k] == Contents[k])
+          || (exists i :: 0 <= i < Data.Length && Data[i] == (k, Contents[k])));
     }
   }
 
